\documentclass[10pt]{article}
\pagestyle{plain}
\textwidth=15.5cm
\textheight=24.0cm
\oddsidemargin=0.3cm
\evensidemargin=0.5cm

\usepackage[utf8]{inputenc}
\usepackage[T2A]{fontenc}
\usepackage[russian]{babel}
\usepackage{amssymb,amsmath, amsthm}
\usepackage{graphicx}
\usepackage[a4paper,bmargin=2.5cm]{geometry}

\voffset=0pt
\headheight=0pt
\headsep=0pt

\begin{document}

\def\chap#1#2{\ \\ {\large\bf#1 \ | \ \tt\scshape#2} \par}

\ \vspace{-1cm}

{\bf
\ \\
\Large\centerline{\scshape Матлог 6.5b}
}\normalsize

Докажем по индукции по $p$. 
\begin{itemize}
    \item База. $p=0$, тогда $p=0 \lor (\exists q. q^\prime = p)$.
    \item Переход. Пусть $p = 0 \lor (\exists q. q^\prime = p)$.
    Тогда для $p^\prime$ $q = p$ и $q^\prime = p^\prime$ (A2).  
\end{itemize}

Доказательство в формальной арифметике: $P = p = 0 \lor \exists q. q^\prime = p$
\begin{enumerate}
    \item $0 = 0$ (теорема)
    \item $0=0 \implies 0 = 0 \lor \exists q. q^\prime = 0$ (добавление ''или'' к 1)
    \item $0 = 0 \lor \exists q. q^\prime = 0$~--- $P[p = 0]$ (MP1,2)
    \item $p^\prime = p^\prime$ (теорема)~--- $(q^\prime = p^\prime)[q=p]$
    \item $(q^\prime = p^\prime)[q=p] \implies \exists q. q^\prime = p^\prime$ (аксиома 12)
    \item $\exists q. q^\prime = p^\prime$ (MP 4,5)
    \item $\exists q. q^\prime = p^\prime \implies (\exists q. q^\prime = p^\prime) \lor p^\prime = 0$ (добавление ''или'' к 6)
    \item $(\exists q. q^\prime = p^\prime) \lor p^\prime = 0$~--- $P[p=p^\prime]$ (MP 6,7)
    \item $P[p=p^\prime] \implies 0=0 \implies P[p=p^\prime]$ (аксиома 1)
    \item $0=0 \implies P[p=p^\prime]$ (MP)
    \item $(0=0 \implies P[p=p^\prime]) \implies 0=0 \implies \forall p. P[p = p^\prime]$ (правило для $\forall$)
    \item $\forall p. P[p = p^\prime]$ (MP)
    \item $P[p=0] \implies \forall p. P[p=p^\prime] \implies (P[p=0] \land \forall p. P[p=p^\prime])$ (введение ''и'')
    \item $P[p=0] \land \forall p. P[p=p^\prime]$ (MP дважды)
    \item $P[p=0] \land \forall p. P[p=p^\prime] \implies P$ (правило индукции)
    \item P
    \item $0=0 \implies P$
    \item $(0=0 \implies P) \implies (0=0 \implies \forall p. P)$
    \item $0=0 \implies \forall p. P$
    \item $\forall p. P$
\end{enumerate}
\end{document}